Ported revisions 7940:7965 from HOL to HOL-Omega. This is to keep HOL-Omega current with the latest HOL developments.

examples/machine-code/compiler/codegen_x86Lib.sml
@@ -19,7 +19,7 @@ fun to_x86_regs () = let
 
 val x86_assign2assembly = let
   fun r i = x86_reg i
-  fun s i = "[esp + " ^ int_to_string (4 * i) ^ "]"
+  fun s i = "[ebp - " ^ int_to_string (4 * i) ^ "]"
   fun address (ASSIGN_ADDRESS_REG i) = "[" ^ r i ^ "]"
     | address (ASSIGN_ADDRESS_OFFSET_ADD (d,i)) = "[" ^ r d ^ " + " ^ Arbnum.toString i ^ "]"
     | address (ASSIGN_ADDRESS_OFFSET_SUB (d,i)) = "[" ^ r d ^ " - " ^ Arbnum.toString i ^ "]"
