src/list/src/listSimps.sml
@@ -297,11 +297,12 @@ in
 end;
 
 val LIST_EQ_ss =
-    simpLib.conv_ss
+  simpLib.name_ss "list EQ"
+   (simpLib.conv_ss
       {name  = "LIST_EQ_SIMP_CONV",
        trace = 2,
        key   = SOME ([],Term `l1:'a list = l2:'a list`),
-       conv  = K (K (CHANGED_CONV LIST_EQ_SIMP_CONV))}
+       conv  = K (K (CHANGED_CONV LIST_EQ_SIMP_CONV))})
 
 end;
 
